vertical composition

compcertox/Encapsulation.v
@@ -147,13 +147,14 @@ Definition semantics_embed {liA liB} (L: semantics liA liB) : liA +-> liB :=
 
 (** ** Simulations *)
 Set Implicit Arguments.
+Require Import Relation_Operators.
 
 Module ST.
 
   Record callconv  {li1 li2} :=
     mk_callconv {
       ccworld : world;
-      match_senv : ccworld -> Genv.symtbl -> Genv.symtbl -> Type;
+      (* match_senv : ccworld -> Genv.symtbl -> Genv.symtbl -> Type; *)
       match_query : ccworld -> query li1 -> query li2 -> Prop;
       match_reply : ccworld -> reply li1 -> reply li2 -> Prop;
     }.
@@ -163,7 +164,7 @@ Module ST.
           (cc: callconv li1 li2) (U V: PSet) : callconv (li1@U) (li2@V) :=
     {|
       ccworld := (ccworld cc * (pset_world U) * (pset_world V))%world;
-      match_senv '(w, u, v) se1 se2 := match_senv cc w se1 se2;
+      (* match_senv '(w, u, v) se1 se2 := match_senv cc w se1 se2; *)
       match_query '(w, u, v) '(q1, uq) '(q2, vq) :=
         match_query cc w q1 q2 /\ u = uq /\ v = vq;
       match_reply '(w, u, v) '(q1, uq) '(q2, vq) :=
@@ -174,8 +175,8 @@ Module ST.
           (cc12: callconv li1 li2) (cc23: callconv li2 li3) :=
     {|
       ccworld := ccworld cc12 * ccworld cc23;
-      match_senv '(w12, w23) se1 se3 :=
-        { se2 & (match_senv cc12 w12 se1 se2 * match_senv cc23 w23 se2 se3)%type };
+      (* match_senv '(w12, w23) se1 se3 := *)
+      (*   { se2 & (match_senv cc12 w12 se1 se2 * match_senv cc23 w23 se2 se3)%type }; *)
       match_query '(w12, w23) q1 q3 :=
       exists q2,
         match_query cc12 w12 q1 q2 /\
@@ -222,10 +223,91 @@ Module ST.
           exists i', exists s2', (Plus L2 s2 t s2' \/ (Star L2 s2 t s2' /\ order i' i)) /\
           exists wA' wB', wA :-> wA' /\ wB *-> wB' /\ match_states wA' wB' i' s1' s2';
       }.
+    Arguments fsim_properties : clear implicits.
 
+    Lemma fsim_simulation':
+      forall L1 L2 index order match_states, fsim_properties L1 L2 index order match_states ->
+      forall i s1 t s1', Step L1 s1 t s1' ->
+      forall wA wB s2, match_states wA wB i s1 s2 ->
+      exists i' wA' wB', wA :-> wA' /\ wB *-> wB' /\
+      ((exists s2', Plus L2 s2 t s2' /\ match_states wA' wB' i' s1' s2')
+      \/ (order i' i /\ t = E0 /\ match_states wA' wB' i' s1' s2)).
+    Proof.
+      intros. exploit @fsim_simulation; eauto.
+      intros (i' & s2' & A & wai & wbi & Hai & Hbi & B).
+      exists i', wai, wbi. repeat split; eauto.
+      destruct A.
+      left; exists s2'; auto.
+      destruct H2. inv H2.
+      right; eauto.
+      left; exists s2'; split; auto. econstructor; eauto.
+    Qed.
+
+    Section SIMULATION_SEQUENCES.
+
+      Context L1 L2 index order match_states
+              (S: fsim_properties L1 L2 index order match_states).
+
+      Lemma simulation_star:
+        forall s1 t s1', Star L1 s1 t s1' ->
+        forall wA wB i s2, match_states wA wB i s1 s2 ->
+        exists wA' wB' i', exists s2', Star L2 s2 t s2' /\
+        wA :-> wA' /\ wB *-> wB' /\ match_states wA' wB' i' s1' s2'.
+      Proof.
+        induction 1; intros.
+        eexists _, _, i; exists s2; repeat split; auto. apply star_refl.
+        reflexivity. reflexivity. assumption.
+        exploit fsim_simulation; eauto.
+        intros (i' & s2' & A & wai & wbi & Hai & Hbi & B).
+        exploit IHstar; eauto.
+        intros (waj & wbj & i'' & s2'' & Hx & Haj & Hbj & C).
+        exists waj, wbj, i''; exists s2''; repeat split; auto.
+        eapply star_trans; eauto.
+        intuition auto. apply plus_star; auto.
+        all: etransitivity; eauto.
+      Qed.
+
+      Lemma simulation_plus:
+        forall s1 t s1', Plus L1 s1 t s1' ->
+        forall wA wB i s2, match_states wA wB i s1 s2 ->
+        exists wA' wB' i', wA :-> wA' /\ wB *-> wB' /\
+        ((exists s2', Plus L2 s2 t s2' /\ match_states wA' wB' i' s1' s2') \/
+        clos_trans _ order i' i /\ t = E0 /\ match_states wA' wB' i' s1' s2).
+      Proof.
+        induction 1 using plus_ind2; intros.
+        (* base case *)
+        - exploit fsim_simulation'; eauto.
+          intros (i' & wai & wbi & Hai & Hbi & A).
+          exists wai, wbi, i'. repeat split; eauto.
+          destruct A.
+          left; auto.
+          right; intuition.
+        (* inductive case *)
+        - exploit fsim_simulation'; eauto.
+          intros (i' & wai & wbi & Hai & Hbi & A).
+          destruct A as [[s2' [A B]] | [A [B C]]].
+          + exploit simulation_star. apply plus_star; eauto. eauto.
+            intros (waj & wbj & i'' & s2'' & P & Haj & Hbj & Q).
+            exists waj, wbj, i''. repeat split. 1-2: etransitivity; eauto.
+            left; exists s2''; split; auto. eapply plus_star_trans; eauto.
+
+          + exploit IHplus; eauto.
+            intros (waj & wbj & i'' & Haj & Hbj & P).
+            destruct P as [[s2'' [P Q]] | [P [Q R]]].
+            * subst. simpl.
+              exists waj, wbj, i''. repeat split. 1-2: etransitivity; eauto.
+              left; exists s2''; auto.
+            * subst. simpl.
+              exists waj, wbj, i''. repeat split. 1-2: etransitivity; eauto.
+              right; intuition auto.
+              eapply t_trans; eauto. eapply t_step; eauto.
+      Qed.
+
+    End SIMULATION_SEQUENCES.
   End FSIM.
 
   Arguments fsim_properties {_ _} _ {_ _} _ _ _ _ {_ _} L1 L2 index order match_states.
+
   Record fsim_components {liA1 liA2} (ccA: callconv liA1 liA2)
          {liB1 liB2} (ccB: callconv liB1 liB2) L1 L2 :=
     Forward_simulation {
@@ -239,10 +321,10 @@ Module ST.
         fsim_skel: skel L1 = skel L2;
         fsim_initial_world: fsim_invariant (pset_init (ccworld ccA)) (pset_init (ccworld ccB));
         fsim_footprint: forall i, footprint L1 i <-> footprint L2 i;
-        fsim_lts wA wB se1 se2 (Hse: match_senv ccB wB se1 se2):
+        fsim_lts wA wB se:
           fsim_invariant wA wB ->
-          fsim_properties ccA ccB wA wB fsim_invariant (activate L1 se1) (activate L2 se2)
-                        fsim_index fsim_order (fsim_match_states se1 se2 wB Hse);
+          fsim_properties ccA ccB wA wB fsim_invariant (activate L1 se) (activate L2 se)
+                          fsim_index fsim_order (fsim_match_states se);
         fsim_order_wf:
           well_founded fsim_order;
       }.
@@ -266,6 +348,8 @@ End E.
 
 (** ** Properties *)
 
+(** *** Embedding Stateless Simulations *)
+
 Definition callconv_embed {liA liB} (cc: callconv liA liB): ST.callconv liA liB :=
   {|
     ST.ccworld := world_embed (ccworld cc);
@@ -283,6 +367,8 @@ Definition callconv_embed {liA liB} (cc: callconv liA liB): ST.callconv liA liB 
 
 Generalizable All Variables.
 
+(* TODO: we cannot prove this property until we figure out the problem about
+   symbol tables *)
 Lemma fsim_embed `(ccA: callconv liA1 liA2) `(ccB: callconv liB1 liB2) L1 L2:
   forward_simulation ccA ccB L1 L2 ->
   E.forward_simulation (callconv_embed ccA) (callconv_embed ccB)
@@ -290,9 +376,85 @@ Lemma fsim_embed `(ccA: callconv liA1 liA2) `(ccB: callconv liB1 liB2) L1 L2:
 Proof.
 Admitted.
 
-(** *** Composition *)
+(** *** Lifting Simulations with Additional States *)
 
-(** Composition of Stateful Simulations *)
+Section LIFT.
+
+  Context `(ccA: ST.callconv liA1 liA2)
+          `(ccB: ST.callconv liB1 liB2)
+          `(X: ST.fsim_components ccA ccB L1 L2).
+  Context (K1 K2: PSet).
+
+  Lemma st_fsim_lift': ST.forward_simulation
+                        (ST.callconv_lift ccA K1 K2)
+                        (ST.callconv_lift ccB K1 K2)
+                        (L1@K1) (L2@K2).
+  Proof.
+    constructor.
+    eapply ST.Forward_simulation with
+      (ST.fsim_order X)
+      (fun se '(wa, k1a, k2a) '(wb, k1b, k2b) i '(s1, k1) '(s2, k2) =>
+         ST.fsim_match_states X se wa wb i s1 s2 /\
+           k1a = k1 /\ k1b = k1 /\ k2a = k2 /\ k2b = k2)
+      (fun '(wa, k1a, k2a) '(wb, k1b, k2b) => ST.fsim_invariant X wa wb /\ k1a = k1b /\ k2a = k2b).
+    - intros [[wa k1a] k2a] [[wb k1b] k2b] (INV & -> & ->) [[wb' k1b'] k2b'] W.
+      destruct W as [[W U] V]. inv U. inv V. repeat split; eauto.
+      eapply ST.fsim_invariant_env_step; eauto.
+    - apply X.
+    - cbn. repeat split; eauto. apply X.
+    - intros i. cbn. apply X.
+    - intros [[wa k1a] k2a] [[wb k1b] k2b] se (I & -> & ->). split; cbn.
+      + intros. prod_crush. subst.
+        pose proof (ST.fsim_lts X _ _ se I).
+        edestruct @ST.fsim_match_initial_states as (idx & s' & Hs' & Hs); eauto.
+        destruct Hs as (wa' & wb'' & W1 & W2 & HS).
+        eexists idx, (s', _). repeat split; eauto.
+        eexists (wa', _, _), (wb'', _, _). repeat split; eauto.
+      + intros. prod_crush. subst.
+        pose proof (ST.fsim_lts X _ _ se I).
+        edestruct @ST.fsim_match_final_states as (r' & H' & Hr'); eauto.
+        destruct Hr' as (wb' & W & Hr' & INV).
+        eexists (r', _). repeat split; eauto.
+        eexists (wb', _, _). repeat split; eauto.
+      + intros. prod_crush. subst.
+        pose proof (ST.fsim_lts X _ _ se I).
+        edestruct @ST.fsim_match_external as (q' & H' & wa' & WA & Hq' & HH); eauto.
+        eexists (q', _). repeat split; eauto.
+        eexists (wa', _, _). repeat split; eauto.
+        intros. prod_crush. subst.
+        edestruct HH as (i' & s2' & Haft & Hs); eauto.
+        destruct Hs as (wa'' & wb' & WA' & WB & HS).
+        eexists i', (s2', _). repeat split; eauto.
+        eexists (wa'', _, _), (wb', _, _). repeat split; eauto.
+      + intros. prod_crush. subst.
+        pose proof (ST.fsim_lts X _ _ se I).
+        edestruct @ST.fsim_simulation as (idx' & s2' & Hs2' & Hs'); eauto.
+        destruct Hs' as (wa' & wb' & WA & WB & HS).
+        destruct Hs2'.
+        * eexists idx', (s2', _). split.
+          -- left. apply lifting_step_plus; eauto.
+          -- eexists (wa', _, _), (wb', _, _).
+             repeat split; eauto.
+        * eexists idx', (s2', _). split.
+          -- right. split. apply lifting_step_star; eauto. all: apply H2.
+          -- eexists (wa', _, _), (wb', _, _).
+             repeat split; eauto.
+    - apply X.
+  Qed.
+
+End LIFT.
+
+Lemma st_fsim_lift `(ccA: ST.callconv liA1 liA2) `(ccB: ST.callconv liB1 liB2)
+      L1 L2 (K1 K2: PSet):
+  ST.forward_simulation ccA ccB L1 L2 ->
+  ST.forward_simulation (ST.callconv_lift ccA K1 K2)
+                        (ST.callconv_lift ccB K1 K2)
+                        (L1@K1) (L2@K2).
+Proof.
+  intros [H]. apply st_fsim_lift'. apply H.
+Qed.
+
+(** *** Composition of Stateful Simulations *)
 
 Section FSIM.
   Context `(ccA: ST.callconv liA1 liA2)
@@ -303,7 +465,7 @@ Section FSIM.
   Context (HL1: ST.fsim_components ccB ccC L1s L1t)
           (HL2: ST.fsim_components ccA ccB L2s L2t)
           (wA : ST.ccworld ccA) (wC: ST.ccworld ccC)
-          (se1 se2: Genv.symtbl).
+          (se: Genv.symtbl).
 
   Variant index := | index1: ST.fsim_index HL1 -> index
                    | index2: ST.fsim_index HL1 -> ST.fsim_index HL2 -> index.
@@ -317,19 +479,19 @@ Section FSIM.
   Inductive match_states: ST.ccworld ccA -> ST.ccworld ccC -> index ->
                           comp_state L1s L2s -> comp_state L1t L2t -> Prop :=
   | match_st1 wa wb wc i1 s1 s1':
-    ST.fsim_match_states HL1 se1 se2 wb wc i1 s1 s1' ->
+    ST.fsim_match_states HL1 se wb wc i1 s1 s1' ->
     ST.fsim_invariant HL2 wa wb ->
     match_states wa wc (index1 i1) (st1 L1s L2s s1) (st1 L1t L2t s1')
   | match_st2 wa wb wc i1 i2 s1 t1 s2 t2 :
-    ST.fsim_match_states HL2 se1 se2 wa wb i2 s2 t2 ->
+    ST.fsim_match_states HL2 se wa wb i2 s2 t2 ->
     (forall r1 r2 (s1' : state L1s) wb',
         wb *-> wb' ->
         ST.match_reply ccB wb' r1 r2 ->
-        after_external (L1s se1) s1 r1 s1' ->
+        after_external (L1s se) s1 r1 s1' ->
         exists (i' : ST.fsim_index HL1) (t1' : state L1t),
-          after_external (L1t se2) t1 r2 t1' /\
+          after_external (L1t se) t1 r2 t1' /\
             exists wb'' wc', wb' :-> wb'' /\ wc *-> wc' /\
-            ST.fsim_match_states HL1 se1 se2 wb'' wc' i' s1' t1') ->
+            ST.fsim_match_states HL1 se wb'' wc' i' s1' t1') ->
     match_states wa wc (index2 i1 i2) (st2 L1s L2s s1 s2) (st2 L1t L2t t1 t2).
 
   Definition inv : ST.ccworld ccA -> ST.ccworld ccC -> Prop :=
@@ -338,13 +500,13 @@ Section FSIM.
   Lemma st_fsim_comp' sk sk':
     inv wA wC ->
     ST.fsim_properties ccA ccC wA wC inv
-                       (comp_semantics' L1s L2s sk se1)
-                       (comp_semantics' L1t L2t sk' se2)
+                       (comp_semantics' L1s L2s sk se)
+                       (comp_semantics' L1t L2t sk' se)
                        index order match_states.
   Proof.
     intros (wB & INV1 & INV2). split; cbn.
     - intros q1 q2 s1 wC' WC Hq H. inv H.
-      pose proof (ST.fsim_lts HL1 _ _ se1 se2 INV1).
+      pose proof (ST.fsim_lts HL1 _ _ se INV1).
       edestruct @ST.fsim_match_initial_states as (idx & s' & Hs' & Hs); eauto.
       destruct Hs as (wB' & wC'' & W1 & W2 & HS).
       exists (index1 idx), (st1 L1t L2t s').
@@ -353,14 +515,14 @@ Section FSIM.
       econstructor. apply HS. eapply ST.fsim_invariant_env_step; eauto.
     - intros wa wb i s1 s2 r1 Hs Hf. inv Hf. inv Hs.
       rename wb into wc. rename wb0 into wb.
-      pose proof (ST.fsim_lts HL1 _ _ se1 se2 INV1).
+      pose proof (ST.fsim_lts HL1 _ _ se INV1).
       edestruct @ST.fsim_match_final_states as (r' & H' & Hr'); eauto.
       destruct Hr' as (wc' & W & Hr' & INV).
       exists r'. split. econstructor; eauto.
       exists wc'. repeat split; eauto.
       exists wb. split; eauto.
     - intros wa wc i s1 s2 q1 Hs H. inv H. inv Hs.
-      pose proof (ST.fsim_lts HL2 _ _ se1 se2 INV2).
+      pose proof (ST.fsim_lts HL2 _ _ se INV2).
       edestruct @ST.fsim_match_external as (q' & H' & wa' & WA & Hq' & HH); eauto.
       exists q'. split. econstructor; eauto.
       exists wa'. repeat split; eauto.
@@ -374,7 +536,7 @@ Section FSIM.
       intros ? ? ? wbx WBX. apply H7. etransitivity; eauto.
     - intros s1 t s2 Hstep wa wc idx t1 Hs.
       inv Hstep; inv Hs.
-      + pose proof (ST.fsim_lts HL1 _ _ se1 se2 INV1).
+      + pose proof (ST.fsim_lts HL1 _ _ se INV1).
         edestruct @ST.fsim_simulation as (idx' & s2' & Hs2' & Hs'); eauto.
         destruct Hs' as (wb' & wc' & WB & WC & HS).
         exists (index1 idx'), (st1 L1t L2t s2'). split.
@@ -383,7 +545,7 @@ Section FSIM.
           split. apply star_internal1. apply H2. constructor; apply H2.
         * exists wa, wc'. repeat split; eauto. reflexivity.
           econstructor; eauto. eapply @ST.fsim_invariant_env_step; eauto.
-      + pose proof (ST.fsim_lts HL2 _ _ se1 se2 INV2).
+      + pose proof (ST.fsim_lts HL2 _ _ se INV2).
         edestruct @ST.fsim_simulation as (idx' & xs2' & Hs2' & Hs'); eauto.
         destruct Hs' as (wa' & wb' & WA & WB & HS).
         exists (index2 i1 idx'), (st2 L1t L2t t0 xs2'). split.
@@ -394,9 +556,9 @@ Section FSIM.
         * exists wa', wc. repeat split; eauto. reflexivity.
           econstructor; eauto.
           intros r1 r2 sr wb'' WB'. apply H7. etransitivity; eauto.
-      + pose proof (ST.fsim_lts HL1 _ _ se1 se2 INV1).
+      + pose proof (ST.fsim_lts HL1 _ _ se INV1).
         edestruct @ST.fsim_match_external as (q' & H' & wb' & WB & Hq' & HH); eauto.
-        pose proof (ST.fsim_lts HL2 _ _ se1 se2 H6).
+        pose proof (ST.fsim_lts HL2 _ _ se H6).
         edestruct @ST.fsim_match_initial_states as (i2 & s' & Hs' & Hs); eauto.
         destruct Hs as (wa' & wb'' & WA & WB' & Hs).
         exists (index2 i1 i2), (st2 L1t L2t s1' s'). split.
@@ -406,7 +568,7 @@ Section FSIM.
           intros r1 r2 sr wb''' WB'' HR Haft.
           specialize (HH r1 r2 sr wb'''). apply HH. etransitivity; eauto.
           exact HR. exact Haft.
-      + pose proof (ST.fsim_lts HL2 _ _ se1 se2 INV2).
+      + pose proof (ST.fsim_lts HL2 _ _ se INV2).
         edestruct @ST.fsim_match_final_states as (r' & H' & Hr'); eauto.
         edestruct Hr' as (wb' & WB & Hr & INV).
         edestruct H8 as (idx & t1 & HH & HX); eauto.
@@ -450,7 +612,7 @@ Section COMP.
       split. apply Ha. apply Hb.
     - cbn. intros i. destruct Ha, Hb.
       rewrite fsim_footprint, fsim_footprint0. reflexivity.
-    - intros wa wc se1 se2 INV. eapply st_fsim_comp'; eauto.
+    - intros wa wc se INV. eapply st_fsim_comp'; eauto.
     - clear - Ha Hb. intros [|].
       + induction (ST.fsim_order_wf Ha f). constructor.
         intros. inv H1. apply H0. auto.
@@ -460,86 +622,7 @@ Section COMP.
 
 End COMP.
 
-(** Lifting Simulations with Additional States *)
-
-Section LIFT.
-
-  Context `(ccA: ST.callconv liA1 liA2)
-          `(ccB: ST.callconv liB1 liB2)
-          `(X: ST.fsim_components ccA ccB L1 L2).
-  Context (K1 K2: PSet).
-
-  Lemma st_fsim_lift': ST.forward_simulation
-                        (ST.callconv_lift ccA K1 K2)
-                        (ST.callconv_lift ccB K1 K2)
-                        (L1@K1) (L2@K2).
-  Proof.
-    constructor.
-    eapply ST.Forward_simulation with
-      (ST.fsim_order X)
-      (fun se1 se2 '(wa, k1a, k2a) '(wb, k1b, k2b) i '(s1, k1) '(s2, k2) =>
-         ST.fsim_match_states X se1 se2 wa wb i s1 s2 /\
-           k1a = k1 /\ k1b = k1 /\ k2a = k2 /\ k2b = k2)
-      (fun '(wa, k1a, k2a) '(wb, k1b, k2b) => ST.fsim_invariant X wa wb /\ k1a = k1b /\ k2a = k2b).
-    - intros [[wa k1a] k2a] [[wb k1b] k2b] (INV & -> & ->) [[wb' k1b'] k2b'] W.
-      destruct W as [[W U] V]. inv U. inv V. repeat split; eauto.
-      eapply ST.fsim_invariant_env_step; eauto.
-    - apply X.
-    - cbn. repeat split; eauto. apply X.
-    - intros i. cbn. apply X.
-    - intros [[wa k1a] k2a] [[wb k1b] k2b] se1 se2 (I & -> & ->). split; cbn.
-      + intros. prod_crush. subst.
-        pose proof (ST.fsim_lts X _ _ se1 se2 I).
-        edestruct @ST.fsim_match_initial_states as (idx & s' & Hs' & Hs); eauto.
-        destruct Hs as (wa' & wb'' & W1 & W2 & HS).
-        eexists idx, (s', _). repeat split; eauto.
-        eexists (wa', _, _), (wb'', _, _). repeat split; eauto.
-      + intros. prod_crush. subst.
-        pose proof (ST.fsim_lts X _ _ se1 se2 I).
-        edestruct @ST.fsim_match_final_states as (r' & H' & Hr'); eauto.
-        destruct Hr' as (wb' & W & Hr' & INV).
-        eexists (r', _). repeat split; eauto.
-        eexists (wb', _, _). repeat split; eauto.
-      + intros. prod_crush. subst.
-        pose proof (ST.fsim_lts X _ _ se1 se2 I).
-        edestruct @ST.fsim_match_external as (q' & H' & wa' & WA & Hq' & HH); eauto.
-        eexists (q', _). repeat split; eauto.
-        eexists (wa', _, _). repeat split; eauto.
-        intros. prod_crush. subst.
-        edestruct HH as (i' & s2' & Haft & Hs); eauto.
-        destruct Hs as (wa'' & wb' & WA' & WB & HS).
-        eexists i', (s2', _). repeat split; eauto.
-        eexists (wa'', _, _), (wb', _, _). repeat split; eauto.
-      + intros. prod_crush. subst.
-        pose proof (ST.fsim_lts X _ _ se1 se2 I).
-        edestruct @ST.fsim_simulation as (idx' & s2' & Hs2' & Hs'); eauto.
-        destruct Hs' as (wa' & wb' & WA & WB & HS).
-        destruct Hs2'.
-        * eexists idx', (s2', _). split.
-          -- left. apply lifting_step_plus; eauto.
-          -- eexists (wa', _, _), (wb', _, _).
-             repeat split; eauto.
-        * eexists idx', (s2', _). split.
-          -- right. split. apply lifting_step_star; eauto. all: apply H2.
-          -- eexists (wa', _, _), (wb', _, _).
-             repeat split; eauto.
-    - apply X.
-  Qed.
-
-End LIFT.
-
-
-Lemma st_fsim_lift `(ccA: ST.callconv liA1 liA2) `(ccB: ST.callconv liB1 liB2)
-      L1 L2 (K1 K2: PSet):
-  ST.forward_simulation ccA ccB L1 L2 ->
-  ST.forward_simulation (ST.callconv_lift ccA K1 K2)
-                        (ST.callconv_lift ccB K1 K2)
-                        (L1@K1) (L2@K2).
-Proof.
-  intros [H]. apply st_fsim_lift'. apply H.
-Qed.
-
-(** Composition of Components with Encapsulated States *)
+(** *** Composition of Components with Encapsulated States *)
 Section COMP.
   Context `(ccA: ST.callconv liA1 liA2)
           `(ccB: ST.callconv liB1 liB2)
@@ -553,15 +636,13 @@ Section COMP.
 
   Lemma encap_fsim_comp : E.forward_simulation ccA ccC Ls Lt.
   Proof.
-    unfold E.forward_simulation in *.
-    unfold comp_esem in *.
+    unfold E.forward_simulation in *. unfold comp_esem in *.
     apply st_fsim_lift with (K1:=pstate L2s) (K2:=pstate L2t) in HL1.
     exploit @st_fsim_comp. exact HL1. exact HL2.
   Admitted.
-
 End COMP.
 
-(** Compositing Stateful Simulation Conventions *)
+(** *** Composition of Stateful Simulation Conventions *)
 
 Section COMP_FSIM.
 
@@ -571,26 +652,22 @@ Section COMP_FSIM.
   Context (H1: ST.fsim_components ccA1 ccB1 Ls Ln)
           (H2: ST.fsim_components ccA2 ccB2 Ln Lf).
 
-  Inductive compose_fsim_match_states:
-    Genv.symtbl -> Genv.symtbl ->
+  Inductive compose_fsim_match_states: Genv.symtbl ->
     ST.ccworld (ST.cc_compose ccA1 ccA2) ->
     ST.ccworld (ST.cc_compose ccB1 ccB2) ->
     (ST.fsim_index H2 * ST.fsim_index H1) ->
     state Ls -> state Lf -> Prop :=
-  | compose_match_states_intro se1 se2 se3 s1 s2 s3 i1 i2 x wa1 wa2 wb1 wb2:
-    ST.fsim_match_states H1 se1 se2 wa1 wb1 i1 s1 s2 ->
-    ST.fsim_match_states H2 se2 se3 wa2 wb2 i2 s2 s3 ->
-    compose_fsim_match_states se1 se3 (x, wa1, wa2) (Some se2, wb1, wb2)
-                         (i2, i1) s1 s3.
+  | compose_match_states_intro se s1 s2 s3 i1 i2 wa1 wa2 wb1 wb2:
+    ST.fsim_match_states H1 se wa1 wb1 i1 s1 s2 ->
+    ST.fsim_match_states H2 se wa2 wb2 i2 s2 s3 ->
+    compose_fsim_match_states se (wa1, wa2) (wb1, wb2) (i2, i1) s1 s3.
 
   Inductive compose_fsim_inv:
     ST.ccworld (ST.cc_compose ccA1 ccA2) ->
     ST.ccworld (ST.cc_compose ccB1 ccB2) -> Prop :=
-  | compose_fsim_inv_intro ase bse wa1 wa2 wb1 wb2 se2:
-    ST.fsim_invariant H1 wa1 wb1 ->
-    ST.fsim_invariant H2 wa2 wb2 ->
-    bse = Some se2 ->
-    compose_fsim_inv (ase, wa1, wa2) (bse, wb1, wb2).
+  | compose_fsim_inv_intro wa1 wa2 wb1 wb2:
+    ST.fsim_invariant H1 wa1 wb1 -> ST.fsim_invariant H2 wa2 wb2 ->
+    compose_fsim_inv (wa1, wa2) (wb1, wb2).
 
   Lemma st_compose_fsim_components:
     ST.fsim_components (ST.cc_compose ccA1 ccA2)
@@ -618,36 +695,73 @@ Section COMP_FSIM.
     (* 2: { subst ff_index. rewrite X1. rewrite X2. reflexivity. } *)
     (* clear X1 X2. *)
     apply ST.Forward_simulation with ff_order compose_fsim_match_states compose_fsim_inv.
-    - intros [[a wa1] wa2] [[b wb1] wb2] I [[b' wb1'] wb2'] [[X1 X2] X3].
+    - intros [wa1 wa2] [wb1 wb2] I [wb1' wb2'] [X1 X2].
       inv I. econstructor.
       eapply (ST.fsim_invariant_env_step H1); eauto.
       eapply (ST.fsim_invariant_env_step H2); eauto.
-      inv X1. reflexivity.
     - rewrite (ST.fsim_skel H1); apply (ST.fsim_skel H2).
     - econstructor. apply (ST.fsim_initial_world H1).
-      apply (ST.fsim_initial_world). admit.
-    - intros i. rewrite (ST.fsim_footprint H1).
-      apply (ST.fsim_footprint H2).
-    - intros [[x wa1] wa2] [[y wb1] wb2] se1 se3 I. inv I.
-      pose proof (ST.fsim_lts H1 wa1 wb1 se1 se2 H5) as X1.
-      pose proof (ST.fsim_lts H2 wa2 wb2 se2 se3 H8) as X2.
+      apply (ST.fsim_initial_world).
+    - intros i. rewrite (ST.fsim_footprint H1). apply (ST.fsim_footprint H2).
+    - intros [wa1 wa2] [wb1 wb2] se I. inv I.
+      pose proof (ST.fsim_lts H1 wa1 wb1 se H4) as X1.
+      pose proof (ST.fsim_lts H2 wa2 wb2 se H6) as X2.
       constructor.
-      + intros q1 q3 s1 ((ose & wb1') & wb2') ((WSE & WB1) & WB2) (q2 & Hq12 & Hq23) Hi.
-        inv WSE.
+      + intros q1 q3 s1 (wb1' & wb2') (WB1 & WB2) (q2 & Hq12 & Hq23) Hi.
         edestruct (@ST.fsim_match_initial_states liAs) as (i & s2 & A & B); eauto.
         edestruct (@ST.fsim_match_initial_states liAn) as (i' & s3 & C & D); eauto.
         destruct B as (wa1' & wb1'' & WA1 & WB1' & B).
         destruct D as (wa2' & wb2'' & WA2 & WB2' & D).
         eexists (i', i), s3. split; eauto.
-        eexists (x, wa1', wa2'), (Some se2, wb1'', wb2''). repeat split; eauto.
+        eexists (wa1', wa2'), (wb1'', wb2''). repeat split; eauto.
         econstructor; eauto.
-      + intros ((a & wa1') & wa2') ((b & wb1') & wb2') (i2, i1) s1 s3 r1 Hs H.
+      + intros (wa1' & wa2') (wb1' & wb2') (i2, i1) s1 s3 r1 Hs H.
         inv Hs.
-        edestruct (@ST.fsim_match_final_states liAs) as (r2 & Hr2 & Hr12); eauto.
-        edestruct (@fsim_match_final_states liA2) as (r3 & Hr3 & Hr23); eauto.
-
-
-
+        edestruct (@ST.fsim_match_final_states liAs) as (r2 & Hr2 & A); eauto.
+        edestruct (@ST.fsim_match_final_states liAn) as (r3 & Hr3 & B); eauto.
+        destruct A as (wb1'' & WB1' & R1 & I1).
+        destruct B as (wb2'' & WB2' & R2 & I2).
+        exists r3. repeat split; eauto.
+        exists (wb1'', wb2''). repeat split; eauto.
+        econstructor; eauto.
+      + intros (wa1' & wa2') (wb1' & wb2') (i2, i1) s1 s3 q1 Hs H.
+        inv Hs.
+        edestruct (@ST.fsim_match_external liAs) as (q2 & Hq2 & wax & Hwx & Hq12 & Hk12); eauto.
+        edestruct (@ST.fsim_match_external liAn) as (q3 & Hq3 & way & Hwy & Hq23 & Hk23); eauto.
+        exists q3. repeat split; eauto. exists (wax, way). repeat split; eauto.
+        econstructor; eauto.
+        intros r1 r3 s1' (wai, waj) (Hwi & Hwj) (r2 & Hr12 & Hr23) HH.
+        edestruct Hk12 as (i2' & s2' & Hs2' & wam & wbm & Ham & Hbm & Hm); eauto.
+        edestruct Hk23 as (i1' & s3' & Hs3' & wan & wbn & Han & Hbn & Hn); eauto.
+        eexists (_, _), _. repeat split; eauto.
+        eexists (_, _), (_, _). repeat split; eauto.
+        econstructor; eauto.
+      + intros s1 t s1' Hstep (wai & waj) (wbi & wbj) (i2, i1) s3 Hs.
+        inv Hs.
+        edestruct (@ST.fsim_simulation' liAs) as (i1' & waii & wbii & Hai & Hbi & Hx); eauto.
+        destruct Hx as [[s2' [A B]] | [A [B C]]].
+        * (* L2 makes one or several steps. *)
+          edestruct (@ST.simulation_plus liAn) as (wak & wbk & i2' & Hak & Hbk & X); eauto.
+          destruct X as [[s3' [P Q]] | [P [Q R]]].
+          -- (* L3 makes one or several steps *)
+            exists (i2', i1'); exists s3'; split.
+            left; eauto.
+            eexists (_, _), (_, _). repeat split; eauto.
+            econstructor; eauto.
+          -- (* L3 makes no step *)
+            exists (i2', i1'); exists s3; split.
+            right; split. subst t; apply star_refl. red. left. auto.
+            eexists (_, _), (_, _). repeat split; eauto.
+            econstructor; eauto.
+        * (* L2 makes no step *)
+          exists (i2, i1'); exists s3; split.
+          right; split. subst t; apply star_refl. red. right. auto.
+            eexists (_, _), (_, _). repeat split; eauto. 1-2: reflexivity.
+            econstructor; eauto.
+    - unfold ff_order.
+      apply wf_lex_ord. apply Transitive_Closure.wf_clos_trans.
+      eapply (ST.fsim_order_wf H2). eapply (ST.fsim_order_wf H1).
+  Qed.
 
 End COMP_FSIM.
 
